platform/tests/RosMasterAMD64.v
@@ -1,0 +1,4 @@
+Require Import Bedrock RosMasterDriver AMD64_gas.
+
+Definition compiled := moduleS E.m.
+Recursive Extraction compiled.
